proof/DDC/Language/SimplePCF.v
@@ -1,0 +1,21 @@
+
+(* Types, expressions, normal forms, values, lifting and substitution *)
+Require Export DDC.Language.SimplePCF.Exp.
+
+(* Typing judgement and environment weakening. *)
+Require Export DDC.Language.SimplePCF.Ty.
+
+(* Substitution of exps in exps preserves typing. *)
+Require Export DDC.Language.SimplePCF.SubstExpExp.
+
+(* Small step evaluation. *)
+Require Export DDC.Language.SimplePCF.Step.
+
+(* A well typed expression is either a value or can take a step. *)
+Require Export DDC.Language.SimplePCF.Progress.
+
+(* When an expression takes a step then the result has the same type. *)
+Require Export DDC.Language.SimplePCF.Preservation.
+
+(* Big step evaluation, and conversion between small step evaluation. *)
+Require Export DDC.Language.SimplePCF.Eval.
