proof/DDC/Language/SimplePCF/SubstExpExp.v
@@ -1,21 +1,21 @@
 
-Require Import TyJudge.
-Require Export Exp.
+Require Import DDC.Language.SimplePCF.Ty.
+Require Export DDC.Language.SimplePCF.Exp.
 
-(* Substitution of values in values. 
+(* Substitution of expressions in expressions preserves typing.
    Inductively, we must reason about performing substitutions at any
    depth, hence we must prove a property about (subst' d x2 x1) instead
    of the weaker (subst x2 x1) which assumes the substitution is taking
    place at top level.
  *)
-Theorem subst_value_value_ix
- :  forall ix e x1 x2 t1 t2
- ,  get  e ix = Some t2
- -> TYPE e           x1 t1
- -> TYPE (drop ix e) x2 t2
- -> TYPE (drop ix e) (substX ix x2 x1) t1.
+Theorem subst_exp_exp_ix
+ :  forall ix te x1 x2 t1 t2
+ ,  get  ix te = Some t2
+ -> TYPE te           x1 t1
+ -> TYPE (delete ix te) x2 t2
+ -> TYPE (delete ix te) (substX ix x2 x1) t1.
 Proof.
- intros. gen ix e x2 t1.
+ intros. gen ix te x2 t1.
  induction x1; intros; simpl; inverts H0; eauto.
 
  Case "XVar".
@@ -26,37 +26,37 @@ Proof.
   SCase "n < ix".
    apply TYVar.
    rewrite <- H4.
-    apply get_drop_above. auto.
+    apply get_delete_above. auto.
 
   SCase "n > ix".
    apply TYVar.
    destruct n.
     false. omega.
     simpl. nnat. rewrite <- H4.
-     apply get_drop_below. omega.
+     apply get_delete_below. omega.
 
  Case "XLam".
   apply TYLam.
-  rewrite drop_rewind.
+  rewrite delete_rewind.
   apply IHx1; auto.
    simpl. apply type_tyenv_weaken. auto.
 
  Case "XFix".
   apply TYFix.
-  rewrite drop_rewind.
+  rewrite delete_rewind.
   apply IHx1; auto.
    simpl. apply type_tyenv_weaken. auto.
 Qed.
 
 
-Theorem subst_value_value
- :  forall tenv x1 x2 t1 t2
- ,  TYPE (tenv :> t2) x1 t1
- -> TYPE tenv         x2 t2 
- -> TYPE tenv (substX 0 x2 x1) t1.
+Theorem subst_exp_exp
+ :  forall te x1 x2 t1 t2
+ ,  TYPE (te :> t2) x1 t1
+ -> TYPE te         x2 t2 
+ -> TYPE te (substX 0 x2 x1) t1.
 Proof. 
- intros tenv x1 x2 t1 t2 Ht1 Ht2.
- lets H: subst_value_value_ix 0 (tenv :> t2).
+ intros te x1 x2 t1 t2 Ht1 Ht2.
+ lets H: subst_exp_exp_ix 0 (te :> t2).
   simpl in H. eauto.
 Qed.
 
