proof/Main.v
@@ -2,8 +2,12 @@
    nice make target to build the proofs. *)
 Require Import DDC.Base.
 
-(* Simply Typed Lambda Calculus (STLC) *).
+(* Simply Typed Lambda Calculus (STLC) *)
 Require Import DDC.Language.Simple.
+
+(* STLC with Fixpoints, Boolean choice and Naturals. *)
+Require Import DDC.Language.SimplePCF.
 
 (* System-F. Like STLC, but with type abstraction and application. *)
 Require Import DDC.Language.SystemF.
+
